@prefix skos: <http://www.w3.org/2004/02/skos/core#> .
@prefix rdfs: <http://www.w3.org/2000/01/rdf-schema#> .
@prefix owl: <http://www.w3.org/2002/07/owl#> .
@prefix isothes: <http://purl.org/iso25964/skos-thes#> .
@prefix sosa: <http://www.w3.org/ns/sosa/> .
@prefix dc: <http://purl.org/dc/terms/> .
@prefix prov: <http://www.w3.org/ns/prov#> .
@prefix foaf: <http://xmlns.com/foaf/0.1/> .
@prefix xsd: <http://www.w3.org/2001/XMLSchema#> .

<http://www.w3.org/ns/sosa/isHostedBy> rdfs:label "in platform"@en .
<http://www.w3.org/ns/sosa/hosts> rdfs:label "has instrument"@en .

<https://vocab.met.no/mmd>
 a skos:ConceptScheme ; 
 dc:title "MMD Vocabulary"@en, "MMD Vokabular"@nb ;
 dc:creator "Øystein Godøy" ;
 dc:created "2021-01-20";
 dc:contributor "Lara Ferrighi", "Trygve Halsne", "Morten Wergeland Hansen";
 dc:publisher "Norwegian Meteorological Institute"@en, "Meteorologisk Institutt"@nb;
 dc:license "https://creativecommons.org/publicdomain/zero/1.0/";
 skos:definition "SKOS concept collections of controlled vocabularies or code lists used within the MET Norway Metadata Format (https://github.com/metno/mmd)."@en, "SKOS konseptsamlinger av kontrollerte vokabularer eller kodelister som brukes i MET Norway Metadata Format (https://github.com/metno/mmd)."@nb .

<https://vocab.met.no/mmd>
  a prov:Entity ; 
  prov:wasDerivedFrom <https://github.com/metno/mmd> ;
  prov:generatedAtTime  "2021-01-20"^^xsd:date;
  prov:wasGeneratedBy <https://orcid.org/0000-0001-5221-1377> .

<https://orcid.org/0000-0001-5221-1377>
  a prov:Person, prov:Agent ; 
  foaf:givenName "Lara Ferrighi"@en ; 
  prov:hadRole dc:contributor ;
  prov:actedOnBehalfOf <https://ror.org/001n36p86> .

<https://ror.org/001n36p86>
  a foaf:Organization, prov:Agent ; 
  foaf:name "Norwegian Meteorological Institute" . 

<https://vocab.met.no/mmd/Use_Constraint>
  a skos:Collection, isothes:ConceptGroup ;
  skos:inScheme <https://vocab.met.no/mmd>; 
  skos:prefLabel "Use Constraint"@en ;
  skos:definition "A controlled vocabulary to be used to describe constraints on the usage of metadata and/or data. Ideally as little constraints as possible is defined. The definitions below relate to Creative Commons."@en ;
  skos:member <https://vocab.met.no/mmd/Use_Constraint/CC0-1.0>, <https://vocab.met.no/mmd/Use_Constraint/CC-BY-4.0>, <https://vocab.met.no/mmd/Use_Constraint/CC-BY-SA-4.0>, <https://vocab.met.no/mmd/Use_Constraint/CC-BY-NC-4.0>, <https://vocab.met.no/mmd/Use_Constraint/CC-BY-NC-SA-4.0>, <https://vocab.met.no/mmd/Use_Constraint/CC-BY-ND-4.0>, <https://vocab.met.no/mmd/Use_Constraint/CC-BY-NC-ND-4.0> .

<https://vocab.met.no/mmd/Use_Constraint/CC0-1.0>
  a skos:Concept ;
  skos:prefLabel "CC0-1.0"@en ;
  skos:altLabel "Creative Commons Zero v1.0 Universal"@en, "CC0 – Creative Commons"@en ;
  skos:exactMatch <https://creativecommons.org/share-your-work/public-domain/cc0/feed/rdf/>, <http://spdx.org/licenses/CC0-1.0>, <https://creativecommons.org/share-your-work/public-domain/cc0/> ;
  skos:definition "The person who associated a work with this deed has dedicated the work to the public domain by waiving all of his or her rights to the work worldwide under copyright law, including all related and neighboring rights, to the extent allowed by law."@en .

<https://vocab.met.no/mmd/Use_Constraint/CC-BY-4.0>
  a skos:Concept ;
  skos:prefLabel "CC-BY-4.0"@en ;
  skos:altLabel "Creative Commons Attribution 4.0 International"@en, "Attribution"@en, "Navngivelse"@nb ;
  skos:exactMatch <http://spdx.org/licenses/CC-BY-4.0>, <https://creativecommons.org/licenses/by/4.0/rdf>, <https://creativecommons.org/licenses/by/4.0/> ;
  skos:definition "This license lets others distribute, remix, adapt, and build upon your work, even commercially, as long as they credit you for the original creation. This is the most accommodating of licenses offered. Recommended for maximum dissemination and use of licensed materials."@en .

<https://vocab.met.no/mmd/Use_Constraint/CC-BY-SA-4.0>
  a skos:Concept ;
  skos:prefLabel "CC-BY-SA-4.0"@en ;
  skos:altLabel "Creative Commons Attribution Share Alike 4.0 International"@en, "Attribution-ShareAlike"@en, "Navngivelse-DelPåSammeVilkår"@nb ;
  skos:exactMatch <http://spdx.org/licenses/CC-BY-SA-4.0>, <https://creativecommons.org/licenses/by-sa/4.0/rdf>, <https://creativecommons.org/licenses/by-sa/4.0/> ;
  skos:definition "This license lets others remix, adapt, and build upon your work even for commercial purposes, as long as they credit you and license their new creations under the identical terms. This license is often compared to “copyleft” free and open source software licenses. All new works based on yours will carry the same license, so any derivatives will also allow commercial use. This is the license used by Wikipedia, and is recommended for materials that would benefit from incorporating content from Wikipedia and similarly licensed projects."@en .

<https://vocab.met.no/mmd/Use_Constraint/CC-BY-NC-4.0>
  a skos:Concept ;
  skos:prefLabel "CC-BY-NC-4.0"@en ;
  skos:altLabel "Creative Commons Attribution Non Commercial 4.0 International"@en, "Attribution-NonCommercial"@en, "Navngivelse-IkkeKommersiell"@nb ;
  skos:exactMatch <http://spdx.org/licenses/CC-BY-NC-4.0>, <https://creativecommons.org/licenses/by-nc/4.0/rdf>, <https://creativecommons.org/licenses/by-nc/4.0/> ;
  skos:definition "This license lets others remix, adapt, and build upon your work non-commercially, and although their new works must also acknowledge you and be non-commercial, they don’t have to license their derivative works on the same terms."@en .

<https://vocab.met.no/mmd/Use_Constraint/CC-BY-NC-SA-4.0>
  a skos:Concept ;
  skos:prefLabel "CC-BY-NC-SA-4.0"@en ;
  skos:altLabel "Creative Commons Attribution Non Commercial Share Alike 4.0 International"@en, "Attribution-NonCommercial-ShareAlike"@en, "Navngivelse-IkkeKommersiell-DelPåSammeVilkår"@nb ;
  skos:exactMatch <http://spdx.org/licenses/CC-BY-NC-SA-4.0>, <https://creativecommons.org/licenses/by-nc-sa/4.0/rdf>, <https://creativecommons.org/licenses/by-nc-sa/4.0/> ;
  skos:definition "This license lets others remix, adapt, and build upon your work non-commercially, as long as they credit you and license their new creations under the identical terms."@en .

<https://vocab.met.no/mmd/Use_Constraint/CC-BY-ND-4.0>
  a skos:Concept ;
  skos:prefLabel "CC-BY-ND-4.0"@en ;
  skos:altLabel "Creative Commons Attribution No Derivatives 4.0 International"@en, "Attribution-NoDerivs"@en, "Navngivelse-IngenBearbeidelse"@nb ;
  skos:exactMatch <http://spdx.org/licenses/CC-BY-ND-4.0>, <https://creativecommons.org/licenses/by-nd/4.0/rdf>, <https://creativecommons.org/licenses/by-nd/4.0/> ;
  skos:definition "This license lets others reuse the work for any purpose, including commercially; however, it cannot be shared with others in adapted form, and credit must be provided to you."@en .

<https://vocab.met.no/mmd/Use_Constraint/CC-BY-NC-ND-4.0>
  a skos:Concept ;
  skos:prefLabel "CC-BY-NC-ND-4.0"@en ;
  skos:altLabel "Creative Commons Attribution Non Commercial No Derivatives 4.0 International"@en, "Attribution-NonCommercial-NoDerivs"@en, "Navngivelse-IkkeKommersiell-IngenBearbeidelser"@nb ;
  skos:exactMatch <http://spdx.org/licenses/CC-BY-NC-ND4.0>, <https://creativecommons.org/licenses/by-nc-nd/4.0/rdf>, <https://creativecommons.org/licenses/by-nc-nd/4.0/> ;
  skos:definition "This license is the most restrictive of our six main licenses, only allowing others to download your works and share them with others as long as they credit you, but they can’t change them in any way or use them commercially."@en .


<https://vocab.met.no/mmd/Dataset_Production_Status>
  a skos:Collection, isothes:ConceptGroup ;
  skos:inScheme <https://vocab.met.no/mmd>; 
  skos:prefLabel "Dataset Production Status"@en ;
  skos:definition "Production status for the dataset."@en ;
  skos:member <https://vocab.met.no/mmd/Dataset_Production_Status/Planned>, <https://vocab.met.no/mmd/Dataset_Production_Status/InWork>, <https://vocab.met.no/mmd/Dataset_Production_Status/Complete>, <https://vocab.met.no/mmd/Dataset_Production_Status/Obsolete> .

<https://vocab.met.no/mmd/Dataset_Production_Status/Planned>
  a skos:Concept ;
  skos:prefLabel "Planned"@en ;
  skos:definition "Refers to data sets to be collected in the future and are thus unavailable at the present time. For Example: The Hydro spacecraft has not been launched, but information on planned data sets may be available."@en .

<https://vocab.met.no/mmd/Dataset_Production_Status/InWork>
  a skos:Concept ;
  skos:prefLabel "In Work"@en ;
  skos:definition "Refers to data sets currently undergoing production or data that is continuously being collected or updated. For Example: data from the AIRS instrument on Aqua is being collected continuously."@en .

<https://vocab.met.no/mmd/Dataset_Production_Status/Complete>
  a skos:Concept ;
  skos:prefLabel "Complete"@en ;
  skos:definition "Refers to data sets in which no updates or further data collection will be made. For Example: Nimbus-7 SMMR data collection has been completed."@en .

<https://vocab.met.no/mmd/Dataset_Production_Status/Obsolete>
  a skos:Concept ;
  skos:prefLabel "Obsolete"@en ;
  skos:definition "A new version of the dataset has been generated. The new version should be used, this is kept for back tracing."@en .


<https://vocab.met.no/mmd/Activity_Type>
  a skos:Collection, isothes:ConceptGroup;
  skos:inScheme <https://vocab.met.no/mmd>; 
  skos:prefLabel "Activity Type"@en ;
  skos:definition "Controlled vocabulary to be used in METAMOD context to describe activity types. Rather than using the term observation type or platform which possibly could describe the nature of observed datasets, activity type is used to filter between both observations and simulations that possibly are describing the same phenomena. Activity types are used to identify the origin of the dataset documented within METAMOD. This is not an identification of the observation platform (e.g. specific vessel, SYNOP station or satellite), but more the nature of the generation process (e.g. simulation, in situ observation, remote sensing etc). It is useful in the context of filtering data when searching for relevant datasets."@en ;
  skos:member <https://vocab.met.no/mmd/Activity_Type/Aircraft>, <https://vocab.met.no/mmd/Activity_Type/SpaceBorneInstrument>, <https://vocab.met.no/mmd/Activity_Type/NumericalSimulation>, <https://vocab.met.no/mmd/Activity_Type/ClimateIndicator>, <https://vocab.met.no/mmd/Activity_Type/InSituLandBasedStation>, <https://vocab.met.no/mmd/Activity_Type/InSituShipBasedStation>, <https://vocab.met.no/mmd/Activity_Type/InSituOceanFixedStation>, <https://vocab.met.no/mmd/Activity_Type/InSituOceanMovingStation>, <https://vocab.met.no/mmd/Activity_Type/InSituIceBasedStation>, <https://vocab.met.no/mmd/Activity_Type/Interview-Questionnaire>, <https://vocab.met.no/mmd/Activity_Type/Maps-Charts-Photographs> .

<https://vocab.met.no/mmd/Activity_Type/Aircraft>
  a skos:Concept ;
  skos:prefLabel "Aircraft"@en ;
  skos:definition "Observations made during a flight trajectory. The observations can include remote sensing instruments, dropsondes or in situ measurements. Both manned and unmanned vehicles are covered by this term. The output is typically a trajectory, but could also be profiles or points."@en .

<https://vocab.met.no/mmd/Activity_Type/SpaceBorneInstrument>
  a skos:Concept ;
  skos:prefLabel "Space Borne Instrument"@en ;
  skos:altLabel "Earth Observation Satellite"@en ;
  skos:definition "Observations or analysed products based upon data from a space borne instrument (typically onboard a satellite). The nature of the output is typically gridded of type imagery or profiles."@en .

<https://vocab.met.no/mmd/Activity_Type/NumericalSimulation>
  a skos:Concept ;
  skos:prefLabel "Numerical Simulation"@en ;
  skos:definition "Data are generated by the use of a numerical simulation of the atmosphere, the ocean, the climate or similar. Statistical analysis is not covered by this."@en .

<https://vocab.met.no/mmd/Activity_Type/ClimateIndicator>
  a skos:Concept ;
  skos:prefLabel "Climate Indicator"@en ;
  skos:definition "This indicates a dataset that has been generated by analysis of some data with the emphasis on being representative in a climate context (e.g. consistent in time). Furthermore, a climate indicator is \"compact\" representation of the feature studied (e.g. the temporal evolution of area covered by sea ice in the Arctic). Climate Indicators are frequently linked to GCOS requirements."@en .

<https://vocab.met.no/mmd/Activity_Type/InSituLandBasedStation>
  a skos:Concept ;
  skos:prefLabel "In Situ Land-based station"@en ;
  skos:altLabel "Land station"@en ;
  skos:hiddenLabel "field_experiment"@en ;
  skos:definition "This is used to tag datasets generated from a site located on land. This can be a permanent (e.g. a SYNOP or TEMP station) or a temporary site (e.g. a field experiment)."@en .

<https://vocab.met.no/mmd/Activity_Type/InSituShipBasedStation>
  a skos:Concept ;
  skos:prefLabel "In Situ Ship-based station"@en ;
  skos:altLabel "Cruise"@en ;
  skos:definition "This is used to identify datasets generated during cruises. Typically it describes a full dataset generated in a context, possibly describing both ocean and atmospheric conditions."@en .

<https://vocab.met.no/mmd/Activity_Type/InSituOceanFixedStation>
  a skos:Concept ;
  skos:prefLabel "In Situ Ocean fixed station"@en ;
  skos:hiddenLabel "Moored instrument"@en ;
  skos:definition "This is used to describe ocean stations that are fixed in space. Typically this is moorings, anchored buoys, oil rigs etc."@en .

<https://vocab.met.no/mmd/Activity_Type/InSituOceanMovingStation>
  a skos:Concept ;
  skos:prefLabel "In Situ Ocean moving station"@en ;
  skos:hiddenLabel "Float"@en ;
  skos:definition "This is used to describe ocean stations that are moving around. Typically this is gliders and drifting buoys."@en .

<https://vocab.met.no/mmd/Activity_Type/InSituIceBasedStation>
  a skos:Concept ;
  skos:prefLabel "In Situ Ice-based station"@en ;
  skos:altLabel "Ice station"@en ;
  skos:hiddenLabel "field_experiment"@en ;
  skos:definition "This is used to tag datasets generated from a site located on drifting sea ice or some other ice sheet (possibly on land but moving). It typically describes a temporary site (e.g. a field experiment). It would also be used to describe ships frozen in ice and drifting e.g. across the Arctic as well as Ice Thethered Platforms (ITP) and Ice Mass Balance Buoys (IMBB)."@en .

<https://vocab.met.no/mmd/Activity_Type/Interview-Questionnaire>
  a skos:Concept ;
  skos:prefLabel "Interview/Questionnaire"@en ;
  skos:altLabel "Interview"@en, "Questionnaire"@en ;
  skos:definition "This is not much used within environmental science, but comes in useful sometimes. It is used to cover the results of interviews and questionnaires especially in interdisciplinary science."@en .

<https://vocab.met.no/mmd/Activity_Type/Maps-Charts-Photographs>
  a skos:Concept ;
  skos:prefLabel "Maps/Charts/Photographs"@en ;
  skos:altLabel "Maps"@en, "Charts"@en, "Photographs"@en ;
  skos:definition "This is used to tag datasets containing imagery or PDF documents. This could e.g. be a time lapse photographic session of a specific site illustrating e.g. snow cover or cloud cover. It can also be used to tag documents or maps describing the nature of a field station. It would then require datasets to be linked (which currently is not supported)."@en .


<https://vocab.met.no/mmd/ISO_Topic_Category>
  a skos:Collection, isothes:ConceptGroup ;
  skos:inScheme <https://vocab.met.no/mmd>; 
  skos:exactMatch <http://vocab.nerc.ac.uk/mmd/P05/current/> ;
  skos:prefLabel "ISO Topic Category"@en ;
  skos:definition "Terms defined by ISO describing data themes."@en ;
  skos:member <https://vocab.met.no/mmd/ISO_Topic_Category/inlandWaters>, <https://vocab.met.no/mmd/ISO_Topic_Category/intelligenceMilitary>, <https://vocab.met.no/mmd/ISO_Topic_Category/climatologyMeteorologyAtmosphere>, <https://vocab.met.no/mmd/ISO_Topic_Category/utilitiesCommunications>, <https://vocab.met.no/mmd/ISO_Topic_Category/farming>, <https://vocab.met.no/mmd/ISO_Topic_Category/imageryBaseMapsEarthCover>, <https://vocab.met.no/mmd/ISO_Topic_Category/structure>, <https://vocab.met.no/mmd/ISO_Topic_Category/health>, <https://vocab.met.no/mmd/ISO_Topic_Category/elevation>, <https://vocab.met.no/mmd/ISO_Topic_Category/society>, <https://vocab.met.no/mmd/ISO_Topic_Category/environment>, <https://vocab.met.no/mmd/ISO_Topic_Category/extraTerrestrial>, <https://vocab.met.no/mmd/ISO_Topic_Category/biota>, <https://vocab.met.no/mmd/ISO_Topic_Category/disaster>, <https://vocab.met.no/mmd/ISO_Topic_Category/transportation>, <https://vocab.met.no/mmd/ISO_Topic_Category/geoscientificInformation>, <https://vocab.met.no/mmd/ISO_Topic_Category/oceans>, <https://vocab.met.no/mmd/ISO_Topic_Category/economy>, <https://vocab.met.no/mmd/ISO_Topic_Category/planningCadastre>, <https://vocab.met.no/mmd/ISO_Topic_Category/location>, <https://vocab.met.no/mmd/ISO_Topic_Category/boundaries> .

<https://vocab.met.no/mmd/ISO_Topic_Category/inlandWaters>
  a skos:Concept ;
  skos:exactMatch <http://vocab.nerc.ac.uk/mmd/P05/current/002/> ;
  skos:definition "Inland water features, drainage systems and characteristics, for example rivers and glaciers, salt lakes, water utilization plans, dams, currents, floods and flood hazards, water quality, hydrographic charts, watersheds, wetlands, hydrography"@en ;
  skos:prefLabel "inlandWaters"@en ;
  skos:altLabel "INLAND WATERS"@en .

<https://vocab.met.no/mmd/ISO_Topic_Category/intelligenceMilitary>
  a skos:Concept ;
  skos:definition "Military bases, structures, activities, for example barracks, training grounds, military transportation, information collection"@en ;
  skos:prefLabel "intelligenceMilitary"@en ;
  skos:altLabel "INTELLIGENCE/MILITARY"@en .

<https://vocab.met.no/mmd/ISO_Topic_Category/climatologyMeteorologyAtmosphere>
  a skos:Concept ;
  skos:exactMatch <http://vocab.nerc.ac.uk/mmd/P05/current/004/> ;
  skos:definition "Processes and phenomena of the atmosphere, for example cloud cover, weather, climate, atmospheric conditions, climate change, precipitation"@en ;
  skos:prefLabel "climatologyMeteorologyAtmosphere"@en ;
  skos:altLabel "CLIMATOLOGY/METEOROLOGY/ATMOSPHERE"@en .

<https://vocab.met.no/mmd/ISO_Topic_Category/utilitiesCommunications>
  a skos:Concept ;
  skos:definition "Energy, water and waste systems and communications infrastructure and services, for example hydroelectricity, geothermal, solar and nuclear sources of energy, water purification and distribution, sewage collection and disposal, electricity and gas distribution, data communication, telecommunication, radio, communication networks"@en ;
  skos:prefLabel "utilitiesCommunications"@en ;
  skos:altLabel "UTILITIES/COMMUNICATIONS"@en .

<https://vocab.met.no/mmd/ISO_Topic_Category/farming>
  a skos:Concept ;
  skos:definition "Rearing of animals or cultivation of plants, for example agriculture, irrigation, aquaculture, plantations, herding, pests and diseases affecting crops and livestock"@en ;
  skos:prefLabel "farming"@en ;
  skos:altLabel "FARMING"@en .

<https://vocab.met.no/mmd/ISO_Topic_Category/imageryBaseMapsEarthCover>
  a skos:Concept ;
  skos:definition "Base maps, for example land/earth cover, topographic maps, imagery, unclassified images, annotations, digital ortho imagery"@en ;
  skos:prefLabel "imageryBaseMapsEarthCover"@en ;
  skos:altLabel "IMAGERY/BASE MAPS/EARTH COVER"@en, "IMAGERYBASEMAPSEARTHCOVER"@en .

<https://vocab.met.no/mmd/ISO_Topic_Category/structure>
  a skos:Concept ;
  skos:definition "Man-made construction, for example buildings, museums, churches, factories, housing, monuments, shops, towers, building footprints, architectural and structural plans"@en ;
  skos:prefLabel "structure"@en ;
  skos:altLabel "STRUCTURE"@en .

<https://vocab.met.no/mmd/ISO_Topic_Category/health>
  a skos:Concept ;
  skos:definition "Health, health services, human ecology, and safety, for example disease and illness, factors affecting health, hygiene, substance abuse, mental and physical health, health services, health care providers, public health"@en ;
  skos:prefLabel "health"@en ;
  skos:altLabel "HEALTH"@en .

<https://vocab.met.no/mmd/ISO_Topic_Category/elevation>
  a skos:Concept ;
  skos:definition "Height above or below sea level, for example altitude, bathymetry, digital elevation models, slope, derived products, DEMs, TINs"@en ;
  skos:prefLabel "elevation"@en ;
  skos:altLabel "ELEVATION"@en .

<https://vocab.met.no/mmd/ISO_Topic_Category/society>
  a skos:Concept ;
  skos:definition "Characteristics of society and culture, for example settlements, housing, anthropology, archaeology, education, traditional beliefs, manners and customs, demographic data, tourism, recreational areas and activities, parks, recreational trails, historical sites, cultural resources, social impact assessments, crime and justice, law enforcement, census information, immigration, ethnicity"@en ;
  skos:prefLabel "society"@en ;
  skos:altLabel "SOCIETY"@en .

<https://vocab.met.no/mmd/ISO_Topic_Category/environment>
  a skos:Concept ;
  skos:definition "Environmental resources, protection and conservation, for example environmental pollution, waste storage and treatment, environmental impact assessment, monitoring environmental risk, nature reserves, landscape, water quality, air quality, environmental modeling"@en ;
  skos:prefLabel "environment"@en ;
  skos:altLabel "ENVIRONMENT"@en .

<https://vocab.met.no/mmd/ISO_Topic_Category/extraTerrestrial>
  a skos:Concept ;
  skos:definition ""@en ;
  skos:prefLabel "extraTerrestrial"@en ;
  skos:altLabel "EXTRA TERRESTRIAL"@en .

<https://vocab.met.no/mmd/ISO_Topic_Category/biota>
  a skos:Concept ;
  skos:definition "Flora or fauna in natural environment, for example wildlife, vegetation, biological sciences, ecology, wilderness, sea life, wetlands, habitat, biological resources "@en ;
  skos:prefLabel "biota"@en ;
  skos:altLabel "BIOTA"@en .

<https://vocab.met.no/mmd/ISO_Topic_Category/disaster>
  a skos:Concept ;
  skos:definition ""@en ;
  skos:prefLabel "disaster"@en ;
  skos:altLabel "DISASTER"@en .

<https://vocab.met.no/mmd/ISO_Topic_Category/transportation>
  a skos:Concept ;
  skos:definition "Means and aids for conveying persons or goods, for example roads, airports/airstrips, shipping routes, tunnels nautical charts, vehicle or vessel location, aeronautical charts, railways"@en ;
  skos:prefLabel "transportation"@en ;
  skos:altLabel "TRANSPORTATION"@en .

<https://vocab.met.no/mmd/ISO_Topic_Category/geoscientificInformation>
  a skos:Concept ;
  skos:definition "Information pertaining to earth sciences, for example geophysical features and processes, geology, minerals, sciences dealing with the composition, structure and origin of the earth's rocks, risks of earthquakes, volcanic activity, landslides, gravity information, soils, permafrost, hydrogeology, groundwater, erosion"@en ;
  skos:prefLabel "geoscientificInformation"@en ;
  skos:altLabel "GEOSCIENTIFIC INFORMATION"@en .

<https://vocab.met.no/mmd/ISO_Topic_Category/oceans>
  a skos:Concept ;
  skos:definition "Features and characteristics of salt water bodies (excluding inland waters), for example tides, tidal waves, coastal information, reefs, maritime, outer continental shelf submerged lands, shoreline"@en ;
  skos:prefLabel "oceans"@en ;
  skos:altLabel "OCEANS"@en .

<https://vocab.met.no/mmd/ISO_Topic_Category/economy>
  a skos:Concept ;
  skos:definition "Economic activities, conditions, and employment, for example production, labor, revenue, business, commerce, industry, tourism and ecotourism, forestry, fisheries, commercial or subsistence hunting, exploration and exploitation of resources such as minerals, oil and gas"@en ;
  skos:prefLabel "economy"@en ;
  skos:altLabel "ECONOMY"@en .

<https://vocab.met.no/mmd/ISO_Topic_Category/planningCadastre>
  a skos:Concept ;
  skos:definition "Information used for appropriate actions for future use of the land, for example land use maps, zoning maps, cadastral surveys, land ownership, parcels, easements, tax maps, federal land ownership status, public land conveyance records"@en ;
  skos:prefLabel "planningCadastre"@en ;
  skos:altLabel "PLANNING CADASTRE"@en .

<https://vocab.met.no/mmd/ISO_Topic_Category/location>
  a skos:Concept ;
  skos:definition "Positional information and services, for example addresses, geodetic networks, geodetic control points, postal zones and services, place names, geographic names"@en ;
  skos:prefLabel "location"@en ;
  skos:altLabel "LOCATION"@en .

<https://vocab.met.no/mmd/ISO_Topic_Category/boundaries>
  a skos:Concept ;
  skos:definition " Legal land descriptions, for example political and administrative boundaries, governmental units, marine boundaries, voting districts, school districts, international boundaries"@en ;
  skos:prefLabel "boundaries"@en ;
  skos:altLabel "BOUNDARIES"@en .


<https://vocab.met.no/mmd/Access_Constraint>
  a skos:Collection, isothes:ConceptGroup ;
  skos:inScheme <https://vocab.met.no/mmd>; 
  skos:prefLabel "Access Constraint"@en ;
  skos:definition "A controlled vocabulary to be used to describe the constraints on accessing specific metadata and/or metadata. This is used to determine the exposure of metadata and data internally and externally. Ideallly all datasets (metadata and data) are freely available, but it is acknowledged that some metadata and data may have restrictions that limits their visibility to specific communities only."@en ;
  skos:member <https://vocab.met.no/mmd/Access_Constraint/Open>, <https://vocab.met.no/mmd/Access_Constraint/RegisteredUsersOnlyAutomatedApproval>, <https://vocab.met.no/mmd/Access_Constraint/RegisteredUsersOnlyManualApproval>, <https://vocab.met.no/mmd/Access_Constraint/RestrictedToACommunity>, <https://vocab.met.no/mmd/Access_Constraint/RestrictedAccessToMetadata> .

<https://vocab.met.no/mmd/Access_Constraint/Open>
  a skos:Concept ;
  skos:prefLabel "Open"@en ;
  skos:altLabel "Free"@en, "Unrestricted"@en ;
  skos:definition "These data are freely available to everyone and can be made available without any restrictions."@en .

<https://vocab.met.no/mmd/Access_Constraint/RegisteredUsersOnlyAutomatedApproval>
  a skos:Concept ;
  skos:prefLabel "Registered users only (automated approval)"@en ;
  skos:definition "These data are available for users as long as they register with name, affiliation, and a valid email address. The verification process can be automated."@en .

<https://vocab.met.no/mmd/Access_Constraint/RegisteredUsersOnlyManualApproval>
  a skos:Concept ;
  skos:prefLabel "Registered users only (manual approval required)"@en ;
  skos:definition "These data are available for users as long as they register with name, affiliation, and a valid email address. The verification process must be manual."@en .

<https://vocab.met.no/mmd/Access_Constraint/RestrictedToACommunity>
  a skos:Concept ;
  skos:prefLabel "Restricted to a community"@en ;
  skos:definition "These data are available for users within a restricted community. This community determines the authorization mechansim to utilise whether this being IP-address, community specific users names or other."@en .

<https://vocab.met.no/mmd/Access_Constraint/RestrictedAccessToMetadata>
  a skos:Concept ;
  skos:prefLabel "Restricted access to metadata"@en ;
  skos:definition "Information on these data MUST NOT be exposed externally. This implies that neither metadata can be exposed externally."@en .


<https://vocab.met.no/mmd/Areas>
  a skos:Collection , isothes:ConceptGroup;
  skos:inScheme <https://vocab.met.no/mmd>; 
  skos:prefLabel "Geographical Areas"@en ;
  skos:definition "Controlled vocabulary to be used in METAMOD context to describe geographical areas. This should be related to GCMD science keywords through altLabel. The definition should contain a unique specification of the area. Historically, METAMOD started out with ocean areas only. Open issues remain on how to best classify land regions."@en ;
  skos:member <https://vocab.met.no/mmd/Areas/Arctic>, <https://vocab.met.no/mmd/Areas/BarentsSea>, <https://vocab.met.no/mmd/Areas/BeaufortSea>, <https://vocab.met.no/mmd/Areas/ChukchiSea>, <https://vocab.met.no/mmd/Areas/DenmarkStrait>, <https://vocab.met.no/mmd/Areas/EastSiberianSea>, <https://vocab.met.no/mmd/Areas/FramStrait>, <https://vocab.met.no/mmd/Areas/GreenlandSea>, <https://vocab.met.no/mmd/Areas/IcelandSea>, <https://vocab.met.no/mmd/Areas/KaraSea>, <https://vocab.met.no/mmd/Areas/LaptevSea>, <https://vocab.met.no/mmd/Areas/NordicSeas>, <https://vocab.met.no/mmd/Areas/NorthernHemisphere>, <https://vocab.met.no/mmd/Areas/NorthSea>, <https://vocab.met.no/mmd/Areas/NorwegianSea>, <https://vocab.met.no/mmd/Areas/WhiteSea> .

<https://vocab.met.no/mmd/Areas/Arctic>
  a skos:Concept ;
  skos:prefLabel "Arctic"@en ;
  skos:altLabel "Central Arctic"@en ;
  skos:closeMatch <http://vocab.nerc.ac.uk/mmd/C16/current/17/>, <http://vocab.nerc.ac.uk/mmd/C19/current/9/>, <http://vocab.nerc.ac.uk/mmd/P30/current/arctic_ocean/> ;
  skos:narrowMatch <http://vocab.nerc.ac.uk/mmd/C16/current/08/> ;
  skos:narrower <https://vocab.met.no/mmd/Areas/WhiteSea>, <https://vocab.met.no/mmd/Areas/NorwegianSea> ;
  skos:definition "This is used to indicate that data are located in the Arctic. The definition of the Arctic may however differ as no unique definition exists. In MetaMod context this should refer to data located nortwards of the Arctic Circle, i.e. 65 degrees North."@en .

<https://vocab.met.no/mmd/Areas/BarentsSea>
  a skos:Concept ;
  skos:prefLabel "Barents Sea"@en ;
  skos:exactMatch <http://vocab.nerc.ac.uk/mmd/C16/current/07/>, <http://vocab.nerc.ac.uk/mmd/C19/current/9_4/>, <http://vocab.nerc.ac.uk/mmd/P30/current/barents_sea/> ;
  skos:definition "This is used to indicate data located in the Barents Sea. The definition of this ocean area may differ as no unique definition exists. In MetaMod context this is usually used to refer to observations within or above the sea. It can also be used to identify observations at islands, but such would preferably be indicated with Svalbard if belonging to these islands. {\"Spatial_Coverage\": { \"Southernmost_latitude\": \"65.5666560048002\", \"Northernmost_latitude\": \"82.2514153220693\", \"Westernmost_longitude\": \"16.2694762982728\", \"Easternmost_longitude\": \"68.9755338269347\" }}"@en .

<https://vocab.met.no/mmd/Areas/BeaufortSea>
  a skos:Concept ;
  skos:prefLabel "Beaufort Sea"@en ;
  skos:definition "This is used to indicate data are located in the Beaufort Sea. The definition of this ocean area may differ as no unique definition exists. In MetaMod context this is usually used to refer to observations within or above the sea. {\"Spatial_Coverage\": { \"Southernmost_latitude\": \"65.6130664819046\", \"Northernmost_latitude\": \"76.348429003534\", \"Westernmost_longitude\": \"-156.645774838244\", \"Easternmost_longitude\": \"-121.763081381975\" }}"@en .

<https://vocab.met.no/mmd/Areas/ChukchiSea>
  a skos:Concept ;
  skos:prefLabel "Chukchi Sea"@en ;
  skos:definition "This is used to indicate data located in the Chukchi Sea. The definition of this ocean area may differ as no unique definition exists. In MetaMod context this is usually used to refer to observations in the ocean, but can also be used for observations on islands in the area. {\"Spatial_Coverage\": { \"Southernmost_latitude\": \"65.9080374652434\", \"Northernmost_latitude\": \"71.6078495972615\", \"Westernmost_longitude\": \"177.493486404419\", \"Easternmost_longitude\": \"-156.526019417522\" }}"@en .

<https://vocab.met.no/mmd/Areas/DenmarkStrait>
  a skos:Concept ;
  skos:prefLabel "Denmark Strait"@en ;
  skos:definition "This is used to indicate data located in the Denmark Strait. That is the strait between Iceland and Greenland, effectively separating the Greenland and Iceland Seas. It is used to identify oceanic observations. "@en .

<https://vocab.met.no/mmd/Areas/EastSiberianSea>
  a skos:Concept ;
  skos:prefLabel "East Siberian Sea"@en ;
  skos:definition "{\"Spatial_Coverage\": { \"Southernmost_latitude\": \"67.7983955527279\", \"Northernmost_latitude\": \"79.0000019038462\", \"Westernmost_longitude\": \"138.401622654881\", \"Easternmost_longitude\": \"180\" }}"@en ;
  skos:broader <http://vocab.nerc.ac.uk/mmd/C19/current/9/> .

<https://vocab.met.no/mmd/Areas/FramStrait>
  a skos:Concept ;
  skos:prefLabel "Fram Strait"@en ;
  skos:definition "This is used to indicate data located in the Fram Strait. That is the strait between Svalbard and Greenland, separating the Arctic Ocean from the Greenland Sea. It is primarily used to identify oceanic observations. {\"Spatial_Coverage\": { \"Southernmost_latitude\": \"76.4421290395782\", \"Northernmost_latitude\": \"81.4523562429474\", \"Westernmost_longitude\": \"-9.76400148921\", \"Easternmost_longitude\": \"16.6184257263662\" }}"@en .

<https://vocab.met.no/mmd/Areas/GreenlandSea>
  a skos:Concept ;
  skos:prefLabel "Greenland Sea"@en ;
  skos:definition "This is used to identify data from the area between the Fram Strait and the Denmark Strait, between Greenland and the Mohn-Sverdrup ridge or the Norwegian Sea. It is primarily used for oceanic observations but may also include observations at Jan Mayen. {\"Spatial_Coverage\": { \"Southernmost_latitude\": \"69.7856946623911\", \"Northernmost_latitude\": \"84.0988786741383\", \"Westernmost_longitude\": \"-36.8873951742225\", \"Easternmost_longitude\": \"17.535040165038\" }}"@en .

<https://vocab.met.no/mmd/Areas/IcelandSea>
  a skos:Concept ;
  skos:prefLabel "Iceland Sea"@en ;
  skos:definition """This is used to identify data from the area west and south of the Denmark Strait. It is also used to identify observations from Iceland unless marked as Arctic.  	{"Spatial_Coverage": { "Southernmost_latitude": "62.3430537642984", "Northernmost_latitude": "74.7432353466058", "Westernmost_longitude": "-33.0122766941186", "Easternmost_longitude": "-4.90382728856863" }}"""@en .

<https://vocab.met.no/mmd/Areas/KaraSea>
  a skos:Concept ;
  skos:prefLabel "Kara Sea"@en ;
  skos:definition "This is used to indicate data from ocean, atmosphere and islands in the Kara Sea. {Spatial_Coverage\": { \"Southernmost_latitude\": \"66.0375447387754\", \"Northernmost_latitude\": \"81.3699065017207\", \"Westernmost_longitude\": \"53.8187152298353\", \"Easternmost_longitude\": \"106.071492680497\" }}"@en .

<https://vocab.met.no/mmd/Areas/LaptevSea>
  a skos:Concept ;
  skos:prefLabel "Laptev Sea"@en ;
  skos:definition "This is used to indicate data from ocean, atmosphere and islands in the Laptev Sea. {\"Spatial_Coverage\": { \"Southernmost_latitude\": \"70.162908594833\", \"Northernmost_latitude\": \"81.2788944213394\", \"Westernmost_longitude\": \"95.2333358094057\", \"Easternmost_longitude\": \"141.63867408902\" }}"@en .

<https://vocab.met.no/mmd/Areas/NordicSeas>
  a skos:Concept ;
  skos:prefLabel "Nordic Seas"@en ;
  skos:definition "This is used to identify the combined area of the Norwegian and the North Seas. It is mainly used to identify oceanic data."@en .

<https://vocab.met.no/mmd/Areas/NorthernHemisphere>
  a skos:Concept ;
  skos:prefLabel "Northern Hemisphere"@en ;
  skos:definition "This is a general classification to be used when the more specific definitions are not suitable."@en .

<https://vocab.met.no/mmd/Areas/NorthSea>
  a skos:Concept ;
  skos:prefLabel "North Sea"@en ;
  skos:exactMatch <http://vocab.nerc.ac.uk/mmd/C16/current/04/>, <http://vocab.nerc.ac.uk/mmd/P30/current/north_sea/> ;
  skos:definition "This is used to identify data from the North Sea. Primarily it is used for oceanic observations as well as observations from platforms. The North Sea is located south of the Norwegian Sea, bordered by the Faroe-Shetland area and the Norwegian coast, all the way down to the continent. {\"Spatial_Coverage\": { \"Southernmost_latitude\": \"49.2182615683599\", \"Northernmost_latitude\": \"63.5822291317627\", \"Westernmost_longitude\": \"-5.11211185909971\", \"Easternmost_longitude\": \"9.98777190749643\" }}"@en .

<https://vocab.met.no/mmd/Areas/NorwegianSea>
  a skos:Concept ;
  skos:prefLabel "Norwegian Sea"@en ;
  skos:exactMatch <http://vocab.nerc.ac.uk/mmd/C16/current/06/>, <http://vocab.nerc.ac.uk/mmd/P30/current/norwegian_sea/>, <https://gcmdservices.gsfc.nasa.gov/kms/concept/91dd3935-a1ae-48ca-b263-9b10ac732372> ;
  skos:broader <https://vocab.met.no/mmd/Areas/Arctic> ;
  skos:definition "This is used to identify data from the North Sea. Primarily it is used for oceanic observations as well as observations from platforms. It is bordered by the Greenland Sea, the Barents Sea, the North Sea and the Faroe-Iceland ridge. {\"Spatial_Coverage\": { \"Southernmost_latitude\": \"57.9767651784406\", \"Northernmost_latitude\": \"78.1219500577069\", \"Westernmost_longitude\": \"-9.02068831025837\", \"Easternmost_longitude\": \"27.0790684243223\" }}"@en .

<https://vocab.met.no/mmd/Areas/WhiteSea>
  a skos:Concept ;
  skos:prefLabel "White Sea"@en ;
  skos:exactMatch <http://vocab.nerc.ac.uk/mmd/C16/current/08/> ;
  skos:broader <https://vocab.met.no/mmd/Areas/Arctic> ;
  skos:definition "This is used to indicate data from ocean, atmosphere and islands in the White Sea. {\"Spatial_Coverage\": { \"Southernmost_latitude\": \"63.1090416470606\", \"Northernmost_latitude\": \"68.7989569132796\", \"Westernmost_longitude\": \"31.8685356938203\", \"Easternmost_longitude\": \"44.8394373774493\" }}"@en .


<https://vocab.met.no/mmd/Platform>
  a skos:Collection, isothes:ConceptGroup ;
  skos:inScheme <https://vocab.met.no/mmd>; 
  skos:prefLabel "Platform"@en ;
  skos:exactMatch <https://gcmd.earthdata.nasa.gov/kms/concepts/concept_scheme/platforms> ;
  skos:definition "This describes the platform used to collect the data."@en ;
  skos:member <https://vocab.met.no/mmd/Platform/Sentinel-1A>, <https://vocab.met.no/mmd/Platform/Sentinel-1B>, <https://vocab.met.no/mmd/Platform/Sentinel-2A>, <https://vocab.met.no/mmd/Platform/Sentinel-2B>, <https://vocab.met.no/mmd/Platform/Sentinel-3A>, <https://vocab.met.no/mmd/Platform/Sentinel-3B>, <https://vocab.met.no/mmd/Platform/Metop-A>, <https://vocab.met.no/mmd/Platform/Metop-B>, <https://vocab.met.no/mmd/Platform/Metop-C>, <https://vocab.met.no/mmd/Platform/NOAA-18>, <https://vocab.met.no/mmd/Platform/NOAA-19>, <https://vocab.met.no/mmd/Platform/NOAA-20>, <https://vocab.met.no/mmd/Platform/SNPP>, <https://vocab.met.no/mmd/Platform/Aqua>, <https://vocab.met.no/mmd/Platform/Terra>, <https://vocab.met.no/mmd/Platform/FY-3D>, <https://vocab.met.no/mmd/Platform/FY-3E> .

<https://vocab.met.no/mmd/Platform/Sentinel-1A>
  a skos:Concept, sosa:Platform  ;
  skos:prefLabel "Sentinel-1A"@en ;
  skos:altLabel "Sentinel-1A"@en ;
  sosa:hosts <https://vocab.met.no/mmd/Instrument/SAR-C> ;  
  skos:narrower <https://vocab.met.no/mmd/Instrument/SAR-C> ;
  skos:definition """Sentinel-1 is the European Radar Observatory, representing the first new space component of the GMES (Global Monitoring for Environment and Security) satellite family, designed and developed by ESA and funded by the EC (European Commission). The Copernicus missions (Sentinel-1, -2, and -3) represent the EU contribution to GEOSS (Global Earth Observation System of Systems). Sentinel-1 is composed of a constellation of two satellites, Sentinel-1A and Sentinel-1B, sharing the same orbital plane with a 180° orbital phasing difference. The mission provides an independent operational capability for continuous radar mapping of the Earth with enhanced revisit frequency, coverage, timeliness and reliability for operational services and applications requiring long time series.
"""@en ;
  dc:source <https://directory.eoportal.org/web/eoportal/satellite-missions/c-missions/copernicus-sentinel-1>;
  rdfs:seeAlso <https://earth.esa.int/web/guest/missions/esa-operational-eo-missions/sentinel-1>, <https://www.wmo-sat.info/oscar/satellites/view/sentinel_1a>;
  skos:exactMatch <http://gcmdservices.gsfc.nasa.gov/kms/concept/c7279e54-f7c1-4ee7-a957-719d6021a3f6> .

<https://vocab.met.no/mmd/Platform/Sentinel-1B>
  a skos:Concept, sosa:Platform  ;
  skos:prefLabel "Sentinel-1B"@en ;
  skos:altLabel "Sentinel-1B"@en ;
  sosa:hosts <https://vocab.met.no/mmd/Instrument/SAR-C> ;  
  skos:narrower <https://vocab.met.no/mmd/Instrument/SAR-C> ;
  skos:definition """Sentinel-1 is the European Radar Observatory, representing the first new space component of the GMES (Global Monitoring for Environment and Security) satellite family, designed and developed by ESA and funded by the EC (European Commission). The Copernicus missions (Sentinel-1, -2, and -3) represent the EU contribution to GEOSS (Global Earth Observation System of Systems). Sentinel-1 is composed of a constellation of two satellites, Sentinel-1A and Sentinel-1B, sharing the same orbital plane with a 180° orbital phasing difference. The mission provides an independent operational capability for continuous radar mapping of the Earth with enhanced revisit frequency, coverage, timeliness and reliability for operational services and applications requiring long time series.
"""@en ;
  dc:source <https://directory.eoportal.org/web/eoportal/satellite-missions/c-missions/copernicus-sentinel-1>;
  rdfs:seeAlso <https://earth.esa.int/web/guest/missions/esa-operational-eo-missions/sentinel-1>, <https://www.wmo-sat.info/oscar/satellites/view/sentinel_1b>;
  skos:exactMatch <http://gcmdservices.gsfc.nasa.gov/kms/concept/9940dbad-1a9a-4858-a0e8-af35b21277e2> .

<https://vocab.met.no/mmd/Platform/Sentinel-2A>
  a skos:Concept, sosa:Platform  ;
  skos:prefLabel "Sentinel-2A"@en ;
  skos:altLabel "Sentinel-2A"@en ;
  sosa:hosts <https://vocab.met.no/mmd/Instrument/MSI> ;  
  skos:definition "Sentinel-2 is a multispectral operational imaging mission within the GMES (Global Monitoring for Environment and Security) program, jointly implemented by the EC (European Commission) and ESA (European Space Agency) for global land observation (data on vegetation, soil and water cover for land, inland waterways and coastal areas, and also provide atmospheric absorption and distortion data corrections) at high resolution with high revisit capability to provide enhanced continuity of data so far provided by SPOT-5 and Landsat-7"@en ;
  dc:source <https://directory.eoportal.org/web/eoportal/satellite-missions/c-missions/copernicus-sentinel-2>;
  rdfs:seeAlso <https://earth.esa.int/web/guest/missions/esa-operational-eo-missions/sentinel-2>, <https://www.wmo-sat.info/oscar/satellites/view/sentinel_2a> ;
  skos:exactMatch <https://gcmdservices.gsfc.nasa.gov/kms/concept/6f1c359b-b1a6-47c1-979e-0689e637fbdc> .

<https://vocab.met.no/mmd/Platform/Sentinel-2B>
  a skos:Concept, sosa:Platform  ;
  skos:prefLabel "Sentinel-2B"@en ;
  skos:altLabel "Sentinel-2B"@en ;
  sosa:hosts <https://vocab.met.no/mmd/Instrument/MSI> ;  
  skos:definition "Sentinel-2 is a multispectral operational imaging mission within the GMES (Global Monitoring for Environment and Security) program, jointly implemented by the EC (European Commission) and ESA (European Space Agency) for global land observation (data on vegetation, soil and water cover for land, inland waterways and coastal areas, and also provide atmospheric absorption and distortion data corrections) at high resolution with high revisit capability to provide enhanced continuity of data so far provided by SPOT-5 and Landsat-7"@en ;
  dc:source <https://directory.eoportal.org/web/eoportal/satellite-missions/c-missions/copernicus-sentinel-2>;
  rdfs:seeAlso <https://earth.esa.int/web/guest/missions/esa-operational-eo-missions/sentinel-2>, <https://www.wmo-sat.info/oscar/satellites/view/sentinel_2b> ;
  skos:exactMatch <https://gcmdservices.gsfc.nasa.gov/kms/concept/f2445400-1981-4ef3-bf7c-f4aa35923ae9> .

<https://vocab.met.no/mmd/Platform/Sentinel-3A>
  a skos:Concept, sosa:Platform  ;
  skos:prefLabel "Sentinel-3A"@en ;
  skos:altLabel "Sentinel-3A"@en ;
  sosa:hosts <https://vocab.met.no/mmd/Instrument/OLCI> , <https://vocab.met.no/mmd/Instrument/SLSTR>, <https://vocab.met.no/mmd/Instrument/MWR> ;  
  skos:definition "The Sentinel-3 (S3) mission of ESA and the EC is one of the elements of the GMES (Global Monitoring for Environment and Security) program, which responds to the requirements for operational and near-real-time monitoring of ocean, land and ice surfaces over a period of 20 years. The topography element of this mission will serve primarily the marine operational users but will also allow the monitoring of sea ice and land ice, as well as inland water surfaces, using novel observation techniques.The Sentinel-3 mission is designed as a constellation of two identical polar orbiting satellites, separated by 180º, for the provision of long-term operational marine and land monitoring services. The operational character of this mission implies a high level of availability of the data products and fast delivery time, which have been important design drivers for the mission."@en ;
  dc:source <https://directory.eoportal.org/web/eoportal/satellite-missions/c-missions/copernicus-sentinel-3>;
  rdfs:seeAlso <https://earth.esa.int/web/guest/missions/esa-eo-missions/sentinel-3>, <https://www.wmo-sat.info/oscar/satellites/view/sentinel_3a> ;
  skos:exactMatch <https://gcmdservices.gsfc.nasa.gov/kms/concept/5449d87b-5573-450f-8acb-2fdfeab3c8ce> .

<https://vocab.met.no/mmd/Platform/Sentinel-3B>
  a skos:Concept, sosa:Platform  ;
  skos:prefLabel "Sentinel-3B"@en ;
  skos:altLabel "Sentinel-3B"@en ;
  sosa:hosts <https://vocab.met.no/mmd/Instrument/OLCI> , <https://vocab.met.no/mmd/Instrument/SLSTR>, <https://vocab.met.no/mmd/Instrument/MWR> ;  
  skos:definition "The Sentinel-3 (S3) mission of ESA and the EC is one of the elements of the GMES (Global Monitoring for Environment and Security) program, which responds to the requirements for operational and near-real-time monitoring of ocean, land and ice surfaces over a period of 20 years. The topography element of this mission will serve primarily the marine operational users but will also allow the monitoring of sea ice and land ice, as well as inland water surfaces, using novel observation techniques.The Sentinel-3 mission is designed as a constellation of two identical polar orbiting satellites, separated by 180º, for the provision of long-term operational marine and land monitoring services. The operational character of this mission implies a high level of availability of the data products and fast delivery time, which have been important design drivers for the mission."@en ;
  dc:source <https://directory.eoportal.org/web/eoportal/satellite-missions/c-missions/copernicus-sentinel-3>;
  rdfs:seeAlso <https://earth.esa.int/web/guest/missions/esa-eo-missions/sentinel-3>, <https://www.wmo-sat.info/oscar/satellites/view/sentinel_3b> ;
  skos:exactMatch <https://gcmdservices.gsfc.nasa.gov/kms/concept/41163801-6aac-43e5-aed7-9f52613a6a73> .

<https://vocab.met.no/mmd/Platform/Metop-A>
  a skos:Concept, sosa:Platform  ;
  skos:prefLabel "Metop-A"@en ;
  skos:altLabel "Meteorological operational satellite - A"@en ;
  sosa:hosts <https://vocab.met.no/mmd/Instrument/AVHRR_3> ; 
  skos:narrower <https://vocab.met.no/mmd/Instrument/AVHRR_3> ; 
  skos:definition "The MetOp series, developed by a consortium of European companies led by the main contractor EADS-Astrium, France, builds on the heritage gained from a successful series of European satellites, including the French space agency’s (CNES) SPOT and ESA’s ERS and Envisat. The satellite consists and two modules: the Payload Module (PLM) and the Service Module (SVM), and a large solar array. The PLM accommodates the whole suite of instruments and associated support equipment. MetOp-A was launched in October 2006 from the Baikonur Cosmodrome in Kazakhstan on a Soyuz/ST Fregat operated by Starsem."@en ;
  dc:source <https://www.esa.int/Applications/Observing_the_Earth/Meteorological_missions/MetOp/About_the_satellite> ;
  rdfs:seeAlso <https://www.wmo-sat.info/oscar/satellites/view/metop-a> ;
  skos:exactMatch <https://gcmdservices.gsfc.nasa.gov/kms/concept/8143808e-1005-4fed-a469-c2bd5f1521bf> .

<https://vocab.met.no/mmd/Platform/Metop-B>
  a skos:Concept, sosa:Platform  ;
  skos:prefLabel "Metop-B"@en ;
  skos:altLabel "Meteorological operational satellite - B"@en ;
  sosa:hosts <https://vocab.met.no/mmd/Instrument/AVHRR_3> ; 
  skos:narrower <https://vocab.met.no/mmd/Instrument/AVHRR_3> ; 
  skos:definition "The MetOp series, developed by a consortium of European companies led by the main contractor EADS-Astrium, France, builds on the heritage gained from a successful series of European satellites, including the French space agency’s (CNES) SPOT and ESA’s ERS and Envisat. The satellite consists and two modules: the Payload Module (PLM) and the Service Module (SVM), and a large solar array. The PLM accommodates the whole suite of instruments and associated support equipment. MetOp-B was launched on 17 September 2012. "@en ;
  dc:source <https://www.esa.int/Applications/Observing_the_Earth/Meteorological_missions/MetOp/About_the_satellite> ;
  rdfs:seeAlso <https://www.wmo-sat.info/oscar/satellites/view/metop-b> ;
  skos:exactMatch <https://gcmdservices.gsfc.nasa.gov/kms/concept/c9f84df0-e807-46e3-8fce-c33e9201fbc2> .

<https://vocab.met.no/mmd/Platform/Metop-C>
  a skos:Concept, sosa:Platform  ;
  skos:prefLabel "Metop-C"@en ;
  skos:altLabel "Meteorological operational satellite - C"@en ;
  sosa:hosts <https://vocab.met.no/mmd/Instrument/AVHRR_3> ; 
  skos:narrower <https://vocab.met.no/mmd/Instrument/AVHRR_3> ; 
  skos:definition "The MetOp series, developed by a consortium of European companies led by the main contractor EADS-Astrium, France, builds on the heritage gained from a successful series of European satellites, including the French space agency’s (CNES) SPOT and ESA’s ERS and Envisat. The satellite consists and two modules: the Payload Module (PLM) and the Service Module (SVM), and a large solar array. The PLM accommodates the whole suite of instruments and associated support equipment. MetOp-C joined MetOp series in orbit in November 2018."@en ;
  dc:source <https://www.esa.int/Applications/Observing_the_Earth/Meteorological_missions/MetOp/About_the_satellite> ;
  rdfs:seeAlso <https://www.wmo-sat.info/oscar/satellites/view/metop-c> ;
  skos:exactMatch <https://gcmdservices.gsfc.nasa.gov/kms/concept/6120cea0-c943-4c7c-bddd-8d8648d58022> .

<https://vocab.met.no/mmd/Platform/NOAA-18>
  a skos:Concept, sosa:Platform  ;
  skos:prefLabel "NOAA-18"@en ;
  skos:altLabel "National Oceanic and Atmospheric Administration - 18"@en ;
  sosa:hosts <https://vocab.met.no/mmd/Instrument/AVHRR_3> ; 
  skos:narrower <https://vocab.met.no/mmd/Instrument/AVHRR_3> ; 
  skos:definition "NOAA 18 continues the fourth-generation of operational, polar orbiting, meteorological satellite series (NOAA K-N) operated by the National Environmental Satellite Service (NESS) of the National Oceanic and Atmospheric Administration (NOAA). NOAA 18 also continues the series of Advanced TIROS-N (ATN) spacecraft begun with the launch of NOAA 8 (NOAA-E) in 1983 but with additional new and improved instrumentation over the NOAA A-J series and a new launch vehicle (Titan II). NOAA 18 will be in an afternoon equator-crossing orbit and is intended to replace NOAA 17 as the prime afternoon spacecraft."@en ;
  dc:source <https://nssdc.gsfc.nasa.gov/nmc/spacecraft/display.action?id=2005-018A> ;
  rdfs:seeAlso <https://www.wmo-sat.info/oscar/satellites/view/noaa_18> ;
  skos:exactMatch <https://gcmdservices.gsfc.nasa.gov/kms/concept/37afee26-f2fd-47df-b8e0-7cccd71e6b8c> .

<https://vocab.met.no/mmd/Platform/NOAA-19>
  a skos:Concept, sosa:Platform  ;
  skos:prefLabel "NOAA-19"@en ;
  skos:altLabel "National Oceanic and Atmospheric Administration - 19"@en ;
  sosa:hosts <https://vocab.met.no/mmd/Instrument/AVHRR_3> ; 
  skos:narrower <https://vocab.met.no/mmd/Instrument/AVHRR_3> ; 
  skos:definition "NOAA 19, or NOAA-N Prime, was launched 06 February 2009 at 10:22 UT aboard a Delta 2 rocket from Vandenberg. The 1440 kg satellite was built by Lockheed Martin Space Systems Company. The NOAA polar operational environmental satellites collect global data on: cloud cover; surface conditions such as ice, snow, and vegetation; atmospheric temperatures; and, moisture, aerosol, and ozone distributions. They also collect and relay information from fixed and moving data platforms"@en ;
  dc:source <https://nssdc.gsfc.nasa.gov/nmc/spacecraft/display.action?id=2009-005A> ; 
  rdfs:seeAlso <https://www.wmo-sat.info/oscar/satellites/view/noaa_19> ;
  skos:exactMatch <https://gcmdservices.gsfc.nasa.gov/kms/concept/b7461b99-2b6f-460a-ae7f-6bb37515684d> .

<https://vocab.met.no/mmd/Platform/NOAA-20>
  a skos:Concept, sosa:Platform  ;
  skos:prefLabel "NOAA-20"@en ;
  skos:altLabel "National Oceanic and Atmospheric Administration - 20"@en ;
  sosa:hosts <https://vocab.met.no/mmd/Instrument/VIIRS> ; 
  skos:narrower <https://vocab.met.no/mmd/Instrument/VIIRS> ; 
  skos:definition "NOAA 20 is the first satellite launched in the Joint Polar Satellite System (JPSS). JPSS will provide global environmental data used in numerical weather prediction models for forecasts, and scientific data used for climate monitoring."@en ;
  dc:source <https://nssdc.gsfc.nasa.gov/nmc/spacecraft/display.action?id=2017-073A> ;
  rdfs:seeAlso <https://www.wmo-sat.info/oscar/satellites/view/noaa_20> ;
  skos:exactMatch <https://gcmdservices.gsfc.nasa.gov/kms/concept/586db0b3-5f94-466e-b7c1-a2dbedc0c1fc> .

<https://vocab.met.no/mmd/Platform/SNPP>
  a skos:Concept, sosa:Platform  ;
  skos:prefLabel "SNPP"@en ;
  skos:altLabel "Suomi National Polar-orbiting Partnership"@en ;
  sosa:hosts <https://vocab.met.no/mmd/Instrument/VIIRS> ; 
  skos:narrower <https://vocab.met.no/mmd/Instrument/VIIRS> ; 
  skos:definition "Suomi National Polar-orbiting Partnership, formerly known as the NPOESS Preparatory Project, will serve as a bridge between the EOS satellites and the forthcoming series of Joint Polar Satellite System (JPSS) satellites. Suomi NPP represents a critical first step in building this next-generation satellite system. The JPSS satellites, previously called the National Polar-orbiting Operational Environmental Satellite System (NPOESS), will be developed by NASA for the National Oceanic and Atmospheric Administration (NOAA). Suomi NPP will carry five science instruments and test key technologies for the JPSS missions. Suomi NPP is the first satellite mission to address the challenge of acquiring a wide range of land, ocean, and atmospheric measurements for Earth system science while simultaneously preparing to address operational requirements for weather forecasting."@en ;
  dc:source <https://www.nasa.gov/mission_pages/NPP/main/index.html> ; 
  rdfs:seeAlso <https://www.wmo-sat.info/oscar/satellites/view/snpp> ;
  skos:exactMatch <https://gcmdservices.gsfc.nasa.gov/kms/concept/85a52725-e6a1-430a-8506-c08c59ef31c7> .

<https://vocab.met.no/mmd/Platform/Aqua>
  a skos:Concept, sosa:Platform  ;
  skos:prefLabel "Aqua"@en ;
  skos:altLabel "Earth Observation System - Aqua"@en ;
  sosa:hosts <https://vocab.met.no/mmd/Instrument/MODIS> ;
  skos:narrower <https://vocab.met.no/mmd/Instrument/MODIS> ;
  skos:definition "Aqua, Latin for water, is a NASA Earth Science satellite mission named for the large amount of information that the mission is collecting about the Earth's water cycle, including evaporation from the oceans, water vapor in the atmosphere, clouds, precipitation, soil moisture, sea ice, land ice, and snow cover on the land and ice. Additional variables also being measured by Aqua include radiative energy fluxes, aerosols, vegetation cover on the land, phytoplankton and dissolved organic matter in the oceans, and air, land, and water temperatures."@en ;
  dc:source <https://aqua.nasa.gov/> ;
  rdfs:seeAlso <https://www.wmo-sat.info/oscar/satellites/view/aqua> ;
  skos:exactMatch <https://gcmdservices.gsfc.nasa.gov/kms/concept/ea7fd15d-190d-43f3-bdd3-75f5d88dc3f8> .

<https://vocab.met.no/mmd/Platform/Terra>
  a skos:Concept, sosa:Platform  ;
  skos:prefLabel "Terra"@en ;
  skos:altLabel "Earth Observation System - Terra"@en ;
  sosa:hosts <https://vocab.met.no/mmd/Instrument/MODIS> ;
  skos:narrower <https://vocab.met.no/mmd/Instrument/MODIS> ;
  skos:definition "Terra explores the connections between Earth's atmosphere, land, snow and ice, ocean, and energy balance to understand Earth's climate and climate change and to map the impact of human activity and natural disasters on communities and ecosystems."@en ;
  dc:source <https://terra.nasa.gov/> ;
  rdfs:seeAlso <https://www.wmo-sat.info/oscar/satellites/view/terra> ;
  skos:exactMatch <https://gcmdservices.gsfc.nasa.gov/kms/concept/80eca755-c564-4616-b910-a4c4387b7c54> .

<https://vocab.met.no/mmd/Platform/FY-3D>
  a skos:Concept, sosa:Platform  ;
  skos:prefLabel "FY-3D"@en ;
  skos:altLabel "Feng-Yun 3D"@en ;
  sosa:hosts <https://vocab.met.no/mmd/Instrument/MERSI-2> ;
  sosa:narrower <https://vocab.met.no/mmd/Instrument/MERSI-2> ;
  skos:definition "The FY-3 series of CMA/NSMC (China Meteorological Administration/National Satellite Meteorological Center) represents the second generation of Chinese polar-orbiting meteorological satellites (follow-on of FY-1 series). The FY-3 series represents a cooperative program between CMA and CNSA (China National Space Administration); it was initially approved in 1998 and entered full-scale development in 1999. Key aspects of the FY-3 satellite series include collecting atmospheric data for intermediate- and long-term weather forecasting and global climate research."@en ;
  dc:source <https://directory.eoportal.org/web/eoportal/satellite-missions/f/fy-3> ; 
  rdfs:seeAlso <https://www.wmo-sat.info/oscar/satellites/view/fy_3d> .

<https://vocab.met.no/mmd/Platform/FY-3E>
  a skos:Concept, sosa:Platform  ;
  skos:prefLabel "FY-3E"@en ;
  skos:altLabel "Feng-Yun 3E"@en ;
  skos:definition "The FY-3 series of CMA/NSMC (China Meteorological Administration/National Satellite Meteorological Center) represents the second generation of Chinese polar-orbiting meteorological satellites (follow-on of FY-1 series). The FY-3 series represents a cooperative program between CMA and CNSA (China National Space Administration); it was initially approved in 1998 and entered full-scale development in 1999. Key aspects of the FY-3 satellite series include collecting atmospheric data for intermediate- and long-term weather forecasting and global climate research."@en ;
  dc:source <https://directory.eoportal.org/web/eoportal/satellite-missions/f/fy-3> ; 
  rdfs:seeAlso <https://www.wmo-sat.info/oscar/satellites/view/fy_3e> .

<https://vocab.met.no/mmd/Instrument>
  a skos:Collection, <http://purl.org/iso25964/skos-thes#ConceptGroup> ;
  skos:inScheme <https://vocab.met.no/mmd>; 
  skos:prefLabel "Instrument"@en ;
  skos:definition "TBW"@en ;
  skos:member <https://vocab.met.no/mmd/Instrument/SAR-C>, <https://vocab.met.no/mmd/Instrument/MSI>, <https://vocab.met.no/mmd/Instrument/OLCI>, <https://vocab.met.no/mmd/Instrument/SLSTR>, <https://vocab.met.no/mmd/Instrument/MWR>, <https://vocab.met.no/mmd/Instrument/VIIRS>, <https://vocab.met.no/mmd/Instrument/AVHRR_3>, <https://vocab.met.no/mmd/Instrument/MERSI-2>, <https://vocab.met.no/mmd/Instrument/MODIS> .

<https://vocab.met.no/mmd/Instrument/SAR-C>
  a skos:Concept, sosa:Sensor ;
  skos:prefLabel "SAR-C"@en ;
  sosa:isHostedBy <https://vocab.met.no/mmd/Platform/Sentinel-1A>, <https://vocab.met.no/mmd/Platform/Sentinel-1B> ;
  skos:broader <https://vocab.met.no/mmd/Platform/Sentinel-1A>, <https://vocab.met.no/mmd/Platform/Sentinel-1B> ;
  skos:narrower <https://vocab.met.no/mmd/Instrument_Modes/SM>, <https://vocab.met.no/mmd/Instrument_Modes/IW>, <https://vocab.met.no/mmd/Instrument_Modes/EW>, <https://vocab.met.no/mmd/Instrument_Modes/WV> ; 
  skos:altLabel "Synthetic Aperture Radar (C-band)"@en, "C-SAR"@en ;
  skos:definition "The C-SAR instrument is an active phased array antenna providing fast scanning in elevation (to cover the large range of incidence angle and to support ScanSAR operation) and in azimuth (to allow use of TOPS technique to meet the required image performance). To meet the polarisation requirements, it has dual channel transmit and receive modules and H/V-polarised pairs of slotted waveguides. It has an internal calibration scheme, where transmit signals are routed into the receiver to allow monitoring of amplitude/phase to facilitate high radiometric stability. SENTINEL-1's metallised carbon-fibre-reinforced-plastic radiating waveguides ensure good radiometric stability even though these elements are not covered by the internal calibration scheme. The digital chirp generator and selectable receive filter bandwidths allow efficient use of on-board storage considering the ground range resolution dependence on incidence angle."@en ;
  dc:source <https://sentinel.esa.int/web/sentinel/technical-guides/sentinel-1-sar/sar-instrument> ;
  rdfs:seeAlso <https://sentinels.copernicus.eu/web/sentinel/user-guides/sentinel-1-sar>, <https://www.wmo-sat.info/oscar/instruments/view/sar_c_sentinel_1> ;
  skos:exactMatch <https://gcmdservices.gsfc.nasa.gov/kms/concept/ed400e7c-229e-48be-9a93-84f2fc864448> .

<https://vocab.met.no/mmd/Instrument/MSI>
  a skos:Concept, sosa:Sensor ;
  skos:prefLabel "MSI"@en ;
  skos:altLabel "Multi-Spectral Imager for Sentinel-2"@en ;
  sosa:isHostedBy <https://vocab.met.no/mmd/Platform/Sentinel-2A>, <https://vocab.met.no/mmd/Platform/Sentinel-2B> ;
  skos:definition "The design of the Multispectral Instrument (MSI) on-board SENTINEL-2 has been driven by the requirement for large swath high geometrical and spectral performance of the measurements. The MSI measures the Earth's reflected radiance in 13 spectral bands from VNIR to SWIR."@en ;
  dc:source <https://sentinel.esa.int/web/sentinel/technical-guides/sentinel-2-msi/msi-instrument> ;
  rdfs:seeAlso <https://www.wmo-sat.info/oscar/instruments/view/msi_sentinel_2a> ;
  skos:exactMatch <https://gcmdservices.gsfc.nasa.gov/kms/concept/fc57a9a0-a287-4bcf-a517-20811b55596b> .

<https://vocab.met.no/mmd/Instrument/OLCI>
  a skos:Concept, sosa:Sensor ;
  skos:prefLabel "OLCI"@en ;
  skos:altLabel "Ocean and Land Colour Imager"@en ;
  sosa:isHostedBy <https://vocab.met.no/mmd/Platform/Sentinel-3A>, <https://vocab.met.no/mmd/Platform/Sentinel-3B> ;
  skos:definition "The OLCI instrument baseline is the successor to ENVISAT MERIS with additional spectral channels, different camera arrangements and simplified on-board processing. The OLCI is a push-broom instrument with five camera modules sharing the field of view. The field of view of the five cameras is arranged in a fan-shaped configuration in the vertical plane, perpendicular to the platform velocity. Each camera has an individual field of view of 14.2° and a 0.6° overlap with its neighbours. The whole field of view is shifted across track by 12.6° away from the sun to minimise the impact of sun glint."@en ;
  dc:source <https://sentinels.copernicus.eu/web/sentinel/technical-guides/sentinel-3-olci/olci-instrument> ; 
  rdfs:seeAlso <https://www.wmo-sat.info/oscar/instruments/view/olci>, <https://sentinel.esa.int/web/sentinel/technical-guides/sentinel-3-olci> ;
  skos:exactMatch <https://gcmdservices.gsfc.nasa.gov/kms/concept/65ed042c-df53-4afb-8b6a-1ea16958015d> .

<https://vocab.met.no/mmd/Instrument/SLSTR>
  a skos:Concept, sosa:Sensor ;
  skos:prefLabel "SLSTR"@en ;
  skos:altLabel "Sea and Land Surface Temperature Radiometer"@en ;
  sosa:isHostedBy <https://vocab.met.no/mmd/Platform/Sentinel-3A>, <https://vocab.met.no/mmd/Platform/Sentinel-3B> ;
  skos:definition "The principal aim of the SLSTR instrument mission on-board Sentinel-3 is to provide a reference Land Surface Temperature and Sea Surface Temperature dataset for climate data records. SLSTR has been developed to retrieve global coverage sea surface skin temperatures with zero bias and an uncertainty of ± 0.3 K for a 5° by 5° latitude–longitude area, having a temporal stability of 0.1 K/decade. The instrument has been designed to fulfil these mission aims."@en ;
  dc:source <https://sentinels.copernicus.eu/web/sentinel/technical-guides/sentinel-3-slstr/instrument> ; 
  rdfs:seeAlso <https://sentinel.esa.int/web/sentinel/technical-guides/sentinel-3-slstr>, <https://www.wmo-sat.info/oscar/instruments/view/slstr> ;
  skos:exactMatch <https://gcmdservices.gsfc.nasa.gov/kms/concept/7204c4d5-b7d0-41af-ba90-61d47c6dc610> .

<https://vocab.met.no/mmd/Instrument/MWR>
  a skos:Concept, sosa:Sensor ;
  skos:prefLabel "MWR"@en ;
  skos:altLabel "Micro-Wave Radiometer"@en ;
  sosa:isHostedBy <https://vocab.met.no/mmd/Platform/Sentinel-3A>, <https://vocab.met.no/mmd/Platform/Sentinel-3B> ;
  skos:definition "The design and specifications of the SENTINEL-3 MWR have been based on those of the Envisat MWR. The instrument will measure brightness temperature at 23.8 GHz and 36.5 GHz covering a bandwidth of 200 MHz in each channel. The lower frequency channel is mostly sensitive to atmospheric water vapour and the higher frequency channel to cloud liquid water. Conceptually, it is a balanced Dicke radiometer for brightness temperatures below the Dicke load temperature. Balancing is achieved by means of a noise injection circuit. For brightness temperatures higher than the Dicke load temperature, a conventional Dicke mode is used. The radiometer employs a single offset reflector of 60 cm diameter and two separate feeds for the two channels. Calibration is achieved through a dedicated horn antenna pointing at the cold sky and the highly stable and precisely monitored internal Dicke load."@en ;
  dc:source <https://sentinel.esa.int/web/sentinel/technical-guides/sentinel-3-altimetry/instrument/mwr> ;
  rdfs:seeAlso <https://sentinel.esa.int/web/sentinel/technical-guides/sentinel-3-altimetry/instrument/mwr>, <https://www.wmo-sat.info/oscar/instruments/view/mwr_sentinel_3> ;
  skos:exactMatch <https://gcmdservices.gsfc.nasa.gov/kms/concept/d81fc4e3-c0b4-4205-82b2-ef2161c169a3> .

<https://vocab.met.no/mmd/Instrument/VIIRS>
  a skos:Concept, sosa:Sensor ;
  skos:prefLabel "VIIRS"@en ;
  skos:altLabel "Visible/Infrared Imager Radiometer Suite"@en ;
  sosa:isHostedBy <https://vocab.met.no/mmd/Platform/SNPP>, <https://vocab.met.no/mmd/Platform/NOAA-20> ;
  skos:broader <https://vocab.met.no/mmd/Platform/SNPP>, <https://vocab.met.no/mmd/Platform/NOAA-20> ;
  skos:definition "The Visible Infrared Imaging Radiometer Suite (VIIRS) instrument collects visible and infrared imagery and global observations of land, atmosphere, cryosphere and oceans. VIIRS features daily multi-band imaging capabilities to support the acquisition of high-resolution atmospheric imagery and other instrument products, including visible and infrared imaging of hurricanes and detection of fires, smoke and atmospheric aerosols. "@en ;
  dc:source <https://www.jpss.noaa.gov/viirs.html> ; 
  rdfs:seeAlso <https://www.wmo-sat.info/oscar/instruments/view/viirs> ;
  skos:exactMatch <https://gcmdservices.gsfc.nasa.gov/kms/concept/dd7c719e-5767-4ceb-b83a-66c1401dab4a> .

<https://vocab.met.no/mmd/Instrument/AVHRR_3>
  a skos:Concept, sosa:Sensor ;
  skos:prefLabel "AVHRR/3"@en ;
  skos:altLabel "Advanced Very High Resolution Radiometer / 3"@en ;
  sosa:isHostedBy <https://vocab.met.no/mmd/Platform/Metop-A>, <https://vocab.met.no/mmd/Platform/Metop-B>, <https://vocab.met.no/mmd/Platform/Metop-C>, <https://vocab.met.no/mmd/Platform/NOAA-18>, <https://vocab.met.no/mmd/Platform/NOAA-19> ;
  skos:broader <https://vocab.met.no/mmd/Platform/Metop-A>, <https://vocab.met.no/mmd/Platform/Metop-B>, <https://vocab.met.no/mmd/Platform/Metop-C>, <https://vocab.met.no/mmd/Platform/NOAA-18>, <https://vocab.met.no/mmd/Platform/NOAA-19> ;
  skos:definition "The Advanced Very High Resolution Radiometer (AVHRR/3) is one of the complement of American instruments provided by the National Oceanic and Atmospheric Administration (NOAA) to fly on MetOp-A, B and C. The AVHRR/3 scans the Earth surface in six spectral bands in the range of 0.58 - 12.5 microns. It provides day and night imaging of land, water and clouds, measures sea surface temperature, ice, snow and vegetation cover."@en ;
  dc:source <https://www.esa.int/Applications/Observing_the_Earth/Meteorological_missions/MetOp/About_AVHRR_3> ;
  rdfs:seeAlso <https://www.wmo-sat.info/oscar/instruments/view/avhrr_3> ;
  skos:exactMatch <https://gcmdservices.gsfc.nasa.gov/kms/concept/87c44e15-54c8-407d-a881-8035a2d5512b> .

<https://vocab.met.no/mmd/Instrument/MERSI-2>
  a skos:Concept, sosa:Sensor ;
  skos:prefLabel "MERSI-2"@en ;
  skos:altLabel "Medium Resolution Spectral Imager -2"@en ;
  sosa:isHostedBy <https://vocab.met.no/mmd/Platform/FY-3D> ; 
  skos:broader <https://vocab.met.no/mmd/Platform/FY-3D> ; 
  skos:definition "MERSI-2 is a 25-channel VIS/IR spectroradiometer (replacing and merging MERSI-1 on FY-3A/3B and VIRR on FY-3A//3B/3C ). Scanning technique: Cross-track: 2048 detectors for channels at 1000 m resolution, or 8192 detectors for channels at 250 m resolution, swath 2900 km; Along-track: ten 10 km lines every 1.5 s. Resolution: 250 m or 1.0 km at s.s.p. (sub-satellite point). Coverage/Cycle: Global coverage once/day (VIS/NIR/SWIR channels), twice/day (MWIR/TIR). "@en ;
  dc:source <https://directory.eoportal.org/web/eoportal/satellite-missions/f/fy-3> ; 
  rdfs:seeAlso <https://www.wmo-sat.info/oscar/instruments/view/mersi_2> .

<https://vocab.met.no/mmd/Instrument/MODIS>
  a skos:Concept, sosa:Sensor ;
  skos:prefLabel "MODIS"@en ;
  skos:altLabel "Moderate-resolution Imaging Spectro-radiometer"@en ;
  sosa:isHostedBy <https://vocab.met.no/mmd/Platform/Terra>, <https://vocab.met.no/mmd/Platform/Aqua> ; 
  skos:broader <https://vocab.met.no/mmd/Platform/Terra>, <https://vocab.met.no/mmd/Platform/Aqua> ; 
  skos:definition "MODIS (or Moderate Resolution Imaging Spectroradiometer) is a key instrument aboard the Terra (originally known as EOS AM-1) and Aqua (originally known as EOS PM-1) satellites. Terra's orbit around the Earth is timed so that it passes from north to south across the equator in the morning, while Aqua passes south to north over the equator in the afternoon. Terra MODIS and Aqua MODIS are viewing the entire Earth's surface every 1 to 2 days, acquiring data in 36 spectral bands, or groups of wavelengths (see MODIS Technical Specifications). These data will improve our understanding of global dynamics and processes occurring on the land, in the oceans, and in the lower atmosphere. MODIS is playing a vital role in the development of validated, global, interactive Earth system models able to predict global change accurately enough to assist policy makers in making sound decisions concerning the protection of our environment."@en ;
  dc:source <https://modis.gsfc.nasa.gov/about/> ;
  rdfs:seeAlso <https://www.wmo-sat.info/oscar/instruments/view/modis>; 
  skos:exactMatch <https://gcmdservices.gsfc.nasa.gov/kms/concept/2878f334-35dc-47a7-a3ae-8c5da1adccd3> .


<https://vocab.met.no/mmd/Operational_Status>
  a skos:Collection, isothes:ConceptGroup ;
  skos:inScheme <https://vocab.met.no/mmd>; 
  skos:prefLabel "Operational Status"@en ;
  skos:definition "Controlled vocabulary to be used in METAMOD context to describe operational status of datasets handled. This is used in filtering of the information. Typically scientific datasets are generated without a temporal perspective and review process. The review process of scientific products is publications in refereed journals or in data citation papers. Experimental, Pre-Operational and Operational are concepts supported by institutions with a committment for a specific delivery over time."@en ;
  skos:member <https://vocab.met.no/mmd/Operational_Status/Operational>, <https://vocab.met.no/mmd/Operational_Status/Pre-Operational>, <https://vocab.met.no/mmd/Operational_Status/Experimental>, <https://vocab.met.no/mmd/Operational_Status/Scientific> .

<https://vocab.met.no/mmd/Operational_Status/Operational>
  a skos:Concept ;
  skos:prefLabel "Operational"@en ;
  skos:definition "This is used to tag datasets that are continously being evaluated and validated. The production of the data is under the responsibility of an authority and follows a review and documentation process. Operational data are generated on a continous basis with a temporal perspective."@en .

<https://vocab.met.no/mmd/Operational_Status/Pre-Operational>
  a skos:Concept ;
  skos:prefLabel "Pre-Operational"@en ;
  skos:definition "This is used to describe data that are under review for becoming the next operational delivery. It is usually produced continously, but not necessarily distributed to users not specifically. It covers the intermediate step between Experimental and Operational."@en .

<https://vocab.met.no/mmd/Operational_Status/Experimental>
  a skos:Concept ;
  skos:prefLabel "Experimental"@en ;
  skos:definition "This is used to describe data that belongs to a development and production chain that provides operational data. It is the first step in the process of becoming operational."@en .

<https://vocab.met.no/mmd/Operational_Status/Scientific>
  a skos:Concept ;
  skos:prefLabel "Scientific"@en ;
  skos:definition """This is used to describe purely scientific products. that is products generated through scientific projects and usually with a limited temporal perspective. 
        """@en .

<https://vocab.met.no/mmd/Collection_Keywords>
  a skos:Collection, isothes:ConceptGroup ;
  skos:inScheme <https://vocab.met.no/mmd>; 
  skos:prefLabel "Collection Keywords"@en ;
  skos:definition "The purpose of this vocabulary is to identify which collection a dataset belong to. This is used to identify sets when serving metadata through e.g. OAI-PMH or to identify which data to present in e.g. a project specific portal when all metadata records are in the same repository."@en ;
  skos:member <https://vocab.met.no/mmd/Collection_Keywords/CC>, <https://vocab.met.no/mmd/Collection_Keywords/ADC>, <https://vocab.met.no/mmd/Collection_Keywords/GCW>, <https://vocab.met.no/mmd/Collection_Keywords/NMDC>, <https://vocab.met.no/mmd/Collection_Keywords/SIOS>, <https://vocab.met.no/mmd/Collection_Keywords/NSDN>, <https://vocab.met.no/mmd/Collection_Keywords/DOKI>, <https://vocab.met.no/mmd/Collection_Keywords/DAM>, <https://vocab.met.no/mmd/Collection_Keywords/ACCESS>, <https://vocab.met.no/mmd/Collection_Keywords/NBS>, <https://vocab.met.no/mmd/Collection_Keywords/APPL>, <https://vocab.met.no/mmd/Collection_Keywords/YOPP>, <https://vocab.met.no/mmd/Collection_Keywords/METNCS>, <https://vocab.met.no/mmd/Collection_Keywords/SESS2018>, <https://vocab.met.no/mmd/Collection_Keywords/SESS2019>, <https://vocab.met.no/mmd/Collection_Keywords/SESS2020>, <https://vocab.met.no/mmd/Collection_Keywords/SIOSCD>, <https://vocab.met.no/mmd/Collection_Keywords/SIOSAP>, <https://vocab.met.no/mmd/Collection_Keywords/CVL> .

<https://vocab.met.no/mmd/Collection_Keywords/CC>
  a skos:Concept ;
  skos:prefLabel "CC"@en ;
  skos:definition "Datasets related to the Cryosphere in the context of the CryoClim project."@en .

<https://vocab.met.no/mmd/Collection_Keywords/ADC>
  a skos:Concept ;
  skos:prefLabel "ADC"@en ;
  rdfs:seeAlso <https://adc.met.no/> ;
  skos:definition "Datasets related to the Arctic Data Centre. This is the fall back collection, but it might be that some datasets are not officially part of the ADC collection and thus should only be searchable, but not exported using OAI-PMH."@en .

<https://vocab.met.no/mmd/Collection_Keywords/GCW>
  a skos:Concept ;
  skos:prefLabel "GCW"@en ;
  skos:definition "Datasets related to the WMO Global Cryosphere Watch."@en .

<https://vocab.met.no/mmd/Collection_Keywords/NMDC>
  a skos:Concept ;
  skos:prefLabel "NMDC"@en ;
  skos:definition "Datasets relevant for the Norwegian Marine Data Centre. This is basically datasets of a marine origin, regardless of whether they are of operational or scientific origin."@en .

<https://vocab.met.no/mmd/Collection_Keywords/SIOS>
  a skos:Concept ;
  skos:prefLabel "SIOS"@en ;
  rdfs:seeAlso <https://sios-svalbard.org> ;
  skos:definition "Datasets related to the Svalbard Integrated Arctic Earth Observing System."@en .

<https://vocab.met.no/mmd/Collection_Keywords/NSDN>
  a skos:Concept ;
  skos:prefLabel "NSDN"@en ;
  skos:definition "Datasets related to the Norwegian Scientific Data Network (NorDataNet)."@en .

<https://vocab.met.no/mmd/Collection_Keywords/DOKI>
  a skos:Concept ;
  skos:prefLabel "DOKI"@en ;
  skos:definition "Datasets related to the national contribution to the International Polar Year."@en .

<https://vocab.met.no/mmd/Collection_Keywords/DAM>
  a skos:Concept ;
  skos:prefLabel "DAM"@en ;
  skos:definition "Datasets in the context of EU FP6 project DAMOCLES."@en .

<https://vocab.met.no/mmd/Collection_Keywords/ACCESS>
  a skos:Concept ;
  skos:prefLabel "ACCESS"@en ;
  skos:definition "Datasets in the context of EU FP7 project ACCESS."@en .

<https://vocab.met.no/mmd/Collection_Keywords/NBS>
  a skos:Concept ;
  skos:prefLabel "NBS"@en ;
  skos:definition "Datasets in the context of National Ground Segment for satellite data. This is primarily Sentinel datasets."@en .

<https://vocab.met.no/mmd/Collection_Keywords/APPL>
  a skos:Concept ;
  skos:prefLabel "APPL"@en ;
  skos:definition "Datasets in the context of EU H2020 project APPLICATE."@en .

<https://vocab.met.no/mmd/Collection_Keywords/YOPP>
  a skos:Concept ;
  skos:prefLabel "YOPP"@en ;
  skos:definition "Datasets in the context of YOPP."@en .

<https://vocab.met.no/mmd/Collection_Keywords/METNCS>
  a skos:Concept ;
  skos:prefLabel "METNCS"@en ;
  skos:definition "Datasets related to the core services at MET Norway."@en .

<https://vocab.met.no/mmd/Collection_Keywords/SESS2018>
  a skos:Concept ;
  skos:prefLabel "SESS2018"@en ;
  rdfs:seeAlso <https://sios-svalbard.org/SESS_Issue1> ;
  skos:definition "Datasets from the State of Environmental Science in Svalbard (SESS) report in 2018."@en .

<https://vocab.met.no/mmd/Collection_Keywords/SESS2019>
  a skos:Concept ;
  skos:prefLabel "SESS2019"@en ;
  rdfs:seeAlso <https://sios-svalbard.org/SESS_Issue2> ;
  skos:definition "Datasets from the State of Environmental Science in Svalbard (SESS) report in 2019."@en .

<https://vocab.met.no/mmd/Collection_Keywords/SESS2020>
  a skos:Concept ;
  skos:prefLabel "SESS2020"@en ;
  rdfs:seeAlso <https://sios-svalbard.org/SESS_Issue3> ;
  skos:definition "Datasets from the State of Environmental Science in Svalbard (SESS) report in 2020."@en .

<https://vocab.met.no/mmd/Collection_Keywords/SIOSCD>
  a skos:Concept ;
  skos:prefLabel "SIOSCD"@en ;
  skos:definition "Datasets that are SIOS Core Data."@en .

<https://vocab.met.no/mmd/Collection_Keywords/SIOSAP>
  a skos:Concept ;
  skos:prefLabel "SIOSAP"@en ;
  rdfs:seeAlso <https://sios-svalbard.org/RIAccess> ;
  skos:definition "Datasets from the SIOS Access Programme."@en .

<https://vocab.met.no/mmd/Collection_Keywords/CVL>
  a skos:Concept ;
  skos:prefLabel "CVL"@en ;
  skos:definition "Datasets from the ESA Cryosphere Virtual Lab."@en .


<https://vocab.met.no/mmd/Instrument_Modes>
  a skos:Collection, <http://purl.org/iso25964/skos-thes#ConceptGroup> ;
  skos:inScheme <https://vocab.met.no/mmd>; 
  skos:prefLabel "Instrument Modes"@en ;
  skos:definition "Instrument Modes for Sentinel-1 (SAR-C)"@en ;
  rdfs:seeAlso <https://sentinels.copernicus.eu/web/sentinel/user-guides/sentinel-1-sar/acquisition-modes> ; 
  skos:member <https://vocab.met.no/mmd/Instrument_Modes/SM>, <https://vocab.met.no/mmd/Instrument_Modes/IW>, <https://vocab.met.no/mmd/Instrument_Modes/EW>, <https://vocab.met.no/mmd/Instrument_Modes/WV> .

<https://vocab.met.no/mmd/Instrument_Modes/SM>
  a skos:Concept ;
  skos:prefLabel "SM"@en ;
  skos:broader <https://vocab.met.no/mmd/Instrument/SAR-C> ;
  skos:narrower <https://vocab.met.no/mmd/Polarisation_Modes/HH>, <https://vocab.met.no/mmd/Polarisation_Modes/VV>, <https://vocab.met.no/mmd/Polarisation_Modes/HH+HV>, <https://vocab.met.no/mmd/Polarisation_Modes/VV+VH>; 
  rdfs:seeAlso <https://sentinels.copernicus.eu/web/sentinel/user-guides/sentinel-1-sar/acquisition-modes/stripmap> ; 
  skos:definition "StripMap. Relates to Sentinel-1"@en .

<https://vocab.met.no/mmd/Instrument_Modes/IW>
  a skos:Concept ;
  skos:prefLabel "IW"@en ;
  skos:broader <https://vocab.met.no/mmd/Instrument/SAR-C> ;
  skos:narrower <https://vocab.met.no/mmd/Polarisation_Modes/HH>, <https://vocab.met.no/mmd/Polarisation_Modes/VV>, <https://vocab.met.no/mmd/Polarisation_Modes/HH+HV>, <https://vocab.met.no/mmd/Polarisation_Modes/VV+VH>; 
  rdfs:seeAlso <https://sentinels.copernicus.eu/web/sentinel/user-guides/sentinel-1-sar/acquisition-modes/interferometric-wide-swath> ; 
  skos:definition "ScanSAR - Interferometric Wide Swath. Relates to Sentinel-1"@en .

<https://vocab.met.no/mmd/Instrument_Modes/EW>
  a skos:Concept ;
  skos:prefLabel "EW"@en ;
  skos:broader <https://vocab.met.no/mmd/Instrument/SAR-C> ;
  skos:narrower <https://vocab.met.no/mmd/Polarisation_Modes/HH>, <https://vocab.met.no/mmd/Polarisation_Modes/VV>, <https://vocab.met.no/mmd/Polarisation_Modes/HH+HV>, <https://vocab.met.no/mmd/Polarisation_Modes/VV+VH>; 
  rdfs:seeAlso <https://sentinels.copernicus.eu/web/sentinel/user-guides/sentinel-1-sar/acquisition-modes/extra-wide-swath> ;
  skos:definition "ScanSAR - Extra-Wide Swath. Relates to Sentinel-1"@en .

<https://vocab.met.no/mmd/Instrument_Modes/WV>
  a skos:Concept ;
  skos:prefLabel "WV"@en ;
  skos:broader <https://vocab.met.no/mmd/Instrument/SAR-C> ;
  skos:narrower <https://vocab.met.no/mmd/Polarisation_Modes/HH>, <https://vocab.met.no/mmd/Polarisation_Modes/VV> ; 
  rdfs:seeAlso <https://sentinels.copernicus.eu/web/sentinel/user-guides/sentinel-1-sar/acquisition-modes/wave> ;
  skos:definition "Wave Mode. Relates to Sentinel-1"@en .

<https://vocab.met.no/mmd/Polarisation_Modes>
  a skos:Collection,  isothes:ConceptGroup;
  skos:inScheme <https://vocab.met.no/mmd>; 
  skos:prefLabel "Polarisation Modes"@en ;
  skos:definition "Polarisation Modes"@en ;
  skos:member <https://vocab.met.no/mmd/Polarisation_Modes/HH>, <https://vocab.met.no/mmd/Polarisation_Modes/VV>, <https://vocab.met.no/mmd/Polarisation_Modes/HH+HV>, <https://vocab.met.no/mmd/Polarisation_Modes/VV+VH> .

<https://vocab.met.no/mmd/Polarisation_Modes/HH>
  a skos:Concept ;
  skos:prefLabel "HH"@en ;
  skos:broader <https://vocab.met.no/mmd/Instrument_Modes/SM>, <https://vocab.met.no/mmd/Instrument_Modes/IW>, <https://vocab.met.no/mmd/Instrument_Modes/EW>, <https://vocab.met.no/mmd/Instrument_Modes/WV> ;  
  skos:definition "Single polarisation mode: Horisontally transmitted and Horisontally received"@en .

<https://vocab.met.no/mmd/Polarisation_Modes/VV>
  a skos:Concept ;
  skos:prefLabel "VV"@en ;
  skos:broader <https://vocab.met.no/mmd/Instrument_Modes/SM>, <https://vocab.met.no/mmd/Instrument_Modes/IW>, <https://vocab.met.no/mmd/Instrument_Modes/EW>, <https://vocab.met.no/mmd/Instrument_Modes/WV> ;  
  skos:definition "Single polarisation mode: Vertically transmitted and Vertically received"@en .

<https://vocab.met.no/mmd/Polarisation_Modes/HH+HV>
  a skos:Concept ;
  skos:prefLabel "HH+HV"@en ;
  skos:broader <https://vocab.met.no/mmd/Instrument_Modes/SM>, <https://vocab.met.no/mmd/Instrument_Modes/IW>, <https://vocab.met.no/mmd/Instrument_Modes/EW> ;  
  skos:definition "Dual polarisation mode: "@en .

<https://vocab.met.no/mmd/Polarisation_Modes/VV+VH>
  a skos:Concept ;
  skos:prefLabel "VV+VH"@en ;
  skos:broader <https://vocab.met.no/mmd/Instrument_Modes/SM>, <https://vocab.met.no/mmd/Instrument_Modes/IW>, <https://vocab.met.no/mmd/Instrument_Modes/EW> ;  
  skos:definition "Dual polarisation mode: "@en .

<https://vocab.met.no/mmd/Product_Types>
  a skos:Collection, isothes:ConceptGroup ;
  skos:inScheme <https://vocab.met.no/mmd>; 
  skos:prefLabel "Product Types"@en ;
  skos:definition ""@en ;
  skos:member <https://vocab.met.no/mmd/Product_Types/SLC>, <https://vocab.met.no/mmd/Product_Types/GRD>, <https://vocab.met.no/mmd/Product_Types/OCN>, <https://vocab.met.no/mmd/Product_Types/S2MSI1C>, <https://vocab.met.no/mmd/Product_Types/S2MSI2A> . 

<https://vocab.met.no/mmd/Product_Types/SLC>
  a skos:Concept ;
  skos:prefLabel "SLC"@en ;
  skos:altLabel "Single Look Complex"@en ;
  skos:definition "Single Look Complex (SLC) products consist of focused SAR data, geo-referenced using orbit and attitude data from the satellite, and provided in slant-range geometry."@en .

<https://vocab.met.no/mmd/Product_Types/GRD>
  a skos:Concept ;
  skos:prefLabel "GRD"@en ;
  skos:altLabel "Ground Range Detected"@en ;
  skos:definition "Ground Range Detected (GRD) products consist of focused SAR data that has been detected, multi-looked and projected to ground range using an Earth ellipsoid model such as WGS84."@en .

<https://vocab.met.no/mmd/Product_Types/OCN>
  a skos:Concept ;
  skos:prefLabel "OCN"@en ;
  skos:altLabel "Ocean"@en ;
  skos:definition "Ocean (OCN) products for wind, wave and currents applications derived from the SAR data."@en .

<https://vocab.met.no/mmd/Product_Types/S2MSI1C>
  a skos:Concept ;
  skos:prefLabel "S2MSI1C"@en ;
  skos:altLabel "Sentinel-2 MSI Level-1C"@en ;
  skos:definition "Ortho-rectified and UTM geo-coded Top-of-Atmosphere Reflectance with sub-pixel multispectral and multi-date registration."@en .

<https://vocab.met.no/mmd/Product_Types/S2MSI2A>
  a skos:Concept ;
  skos:prefLabel "S2MSI2A"@en ;
  skos:altLabel "Sentinel-2 MSI Level-2A"@en ;
  skos:definition "Ortho-rectified and UTM geo-coded Bottom-of-Atmosphere multi-spectral reflectance. Additional outputs are Aerosol Optical Thickness (AOT) map, Water Vapour (WV) map, Scene Classification map together with Quality Indicators data."@en .


<https://vocab.met.no/mmd/Contact_Roles>
  a skos:Collection, isothes:ConceptGroup ;
  skos:inScheme <https://vocab.met.no/mmd>; 
  skos:prefLabel "Contact Roles"@en ;
  skos:definition ""@en ;
  skos:member <https://vocab.met.no/mmd/Contact_Roles/Investigator>, <https://vocab.met.no/mmd/Contact_Roles/TechnicalContact>, <https://vocab.met.no/mmd/Contact_Roles/MetadataAuthor>, <https://vocab.met.no/mmd/Contact_Roles/DataCenterContact> . 

<https://vocab.met.no/mmd/Contact_Roles/Investigator>
  a skos:Concept ;
  skos:prefLabel "Investigator"@en ;
  skos:definition "The person who headed the investigation or experiment that resulted in the acquisition of the data described (i.e., Principal Investigator, Experiment Team Leader) and knows the details on data collection and processing."@en .

<https://vocab.met.no/mmd/Contact_Roles/TechnicalContact>
  a skos:Concept ;
  skos:prefLabel "Technical contact"@en ;
  skos:definition "The person who is knowledgeable about the technical content of the data (quality, processing methods, units, available software for further processing)."@en .

<https://vocab.met.no/mmd/Contact_Roles/MetadataAuthor>
  a skos:Concept ;
  skos:prefLabel "Metadata author"@en ;
  skos:definition "The main responsible person for the generation of the metadata for this dataset. Other people could have been involved, but this is the main contact with regard to the metadata."@en .

<https://vocab.met.no/mmd/Contact_Roles/DataCenterContact>
  a skos:Concept ;
  skos:prefLabel "Data center contact"@en ;
  skos:definition "An individual affiliated with a data center."@en .

<https://vocab.met.no/mmd/Quality_Control>
  a skos:Collection, isothes:ConceptGroup ;
  skos:inScheme <https://vocab.met.no/mmd> ;
  skos:prefLabel "Quality Control"@en ;
  skos:definition "A controlled vocabulary for the level of quality control performed on the dataset/product."@en ;
  skos:member <https://vocab.met.no/mmd/Quality_Control/NoQualityControl>, <https://vocab.met.no/mmd/Quality_Control/BasicQualityControl>, <https://vocab.met.no/mmd/Quality_Control/ExtendedQualityControl>, <https://vocab.met.no/mmd/Quality_Control/ComprehensiveQualityControl> .

<https://vocab.met.no/mmd/Quality_Control/NoQualityControl>
  a skos:Concept ;
  skos:prefLabel "No quality control"@en ;
  skos:definition "No quality control has been performed on the dataset."@en .

<https://vocab.met.no/mmd/Quality_Control/BasicQualityControl>
  a skos:Concept ;
  skos:prefLabel "Basic quality control"@en ;
  skos:definition "A basic quality control has been performed on the dataset. The result of the quality control follows the data as flags."@en .

<https://vocab.met.no/mmd/Quality_Control/ExtendedQualityControl>
  a skos:Concept ;
  skos:prefLabel "Extended quality control"@en ;
  skos:definition "The dataset has undergone basic real time quality control and more advanced quality control. The advanced quality control may include controls on the temporal and spacial scale. The result follows the data as flags."@en .

<https://vocab.met.no/mmd/Quality_Control/ComprehensiveQualityControl>
  a skos:Concept ;
  skos:prefLabel "Comprehensive quality control"@en ;
  skos:definition "The dataset has undergone extensive quality control, including but not limited to basic and advanced automatic controls and regular manual control. The result of the quality control follows the data as flags."@en .

